concurrency/Modular/bst_inst.v
@@ -4,6 +4,7 @@ Require Import VST.atomics.general_locks.
 Require Import Coq.Sets.Ensembles.
 Require Import bst.puretree.
 Require Import bst.bst.
+Require Import bst.dataStruct.
 Require Import VST.atomics.verif_lock_atomic.
 Require Import VST.floyd.library.
 
@@ -12,16 +13,125 @@ Definition Vprog : varspecs.  mk_varspecs prog. Defined.
 
 Definition t_struct_tree := Tstruct _node noattr.
 Definition t_struct_tree_t := Tstruct _tree_t noattr.
-Definition t_struct_node := Tstruct _node_t noattr.
-Definition t_struct_pn := Tstruct _pn noattr.
 
-Definition number2Z (x : number) : Z :=
-  match x with
-    | Finite_Integer y => y
-    | Neg_Infinity => Int.min_signed
-    | Pos_Infinity => Int.max_signed
-  end.
+#[local]Instance my_specific_tree_rep : NodeRep := {
+  node_rep_R := fun tp r g_info g =>
+    EX (ga gb : gname), EX (x : Z), EX (v pa pb : val), EX (locka lockb : val),
+      !!(g_info = Some (Some (x, v)) /\ and (Z.le Int.min_signed x) (Z.le x Int.max_signed) /\
+       is_pointer_or_null pa /\ is_pointer_or_null locka /\
+       is_pointer_or_null pb /\ is_pointer_or_null lockb /\
+          (tc_val (tptr Tvoid) v) /\ key_in_range x r = true) &&
+       data_at Ews t_struct_tree ((Vint (Int.repr x)), (v, (pa, pb))) tp * 
+       malloc_token Ews t_struct_tree tp *
+       in_tree g ga pa locka * in_tree g gb pb lockb
+}.
 
+
+Check node_rep_R.
+Check range.
+(* Spec of findnext function *)
+(* FOUND = 0, NOTFOUND = 1, NULLNEXT = 2 (NULLNEXT = NULL || NEXT ) *)
+Definition findnext_spec :=
+  DECLARE _findNext
+  WITH x: Z, v: val, b: val, p: val, n: val, tp: val, (*,
+       pa: val, pb: val, px: Z, pv: val*) r: range, g: gname, g_info : option (option ghost_info), sh: share, gv: globals
+  PRE [ tptr tvoid, tptr (tptr tvoid), tint ]
+          PROP (writable_share sh(*; is_pointer_or_null pa; is_pointer_or_null pb*) )
+          PARAMS (p; n; Vint (Int.repr x)) GLOBALS (gv)
+          SEP ((* data_at sh (t_struct_tree_t) (p, n) b *)
+            node_rep_R tp r g_info g;
+               field_at sh (t_struct_tree_t) [StructField _t] tp p (* ;
+               data_at sh t_struct_tree (Vint (Int.repr px), (pv, (pa, pb))) tp *)
+               )
+  POST [ tint ]
+  EX (stt: enum), EX (n' : val), EX (next: val),
+         PROP (match stt with
+               | NF => (n' = next)
+               | F => (n' = p)
+               | NN => (n' = p)
+               end)
+        LOCAL (temp ret_temp (enums stt))
+        SEP (match stt with
+             | NF =>
+               ((* data_at sh (t_struct_tree_t) (p, n') b  * *)
+               field_at sh (t_struct_tree_t) [StructField _t] tp p) (* *
+               data_at sh t_struct_tree (Vint (Int.repr px), (pv, (pa, pb))) tp*)  
+             | F =>
+               (field_at sh (t_struct_tree_t) [StructField _t] tp p)
+               (*data_at sh (t_struct_tree_t) (p, n) b )  *
+               field_at sh (t_struct_tree_t) [StructField _t] tp p *
+               data_at sh t_struct_tree (Vint (Int.repr px), (pv, (pa, pb))) tp*)
+             | NN => (field_at sh (t_struct_tree_t) [StructField _t] tp p
+                     (* data_at sh (t_struct_tree_t) (p, n) b *) )
+             end).
+
+Lemma findNext: semax_body Vprog Gprog f_findNext findnext_spec.
+Proof.
+  start_function.
+  (* int y = pn->p->t->key *)
+  forward. 
+  forward. 
+  forward.
+  entailer !. admit.
+  unfold node_rep_R.
+  simpl.
+  Intros ga gb x0 v0 pa pb locka lockb.
+  forward.
+  forward_if. (* if (_x < _y) *)
+  - (* pn->n = pn->p->t->left *)
+    forward. (* t1 = pn->p *)
+    forward. (* t2 = t1->t *)
+    forward. (* t3 = t2->left *)
+    forward.
+    forward.
+    Exists true.
+    Exists pa.
+    entailer !.
+  - forward_if.
+    (* pn->n = pn->p->t->right *)
+    repeat forward.
+    Exists true. Exists pb.
+    entailer !.
+    forward.
+    Exists false.
+    Exists p.
+    entailer !.
+Qed.
+
+
+
+
+(* Spec of findnext function *)
+Definition findnext_spec :=
+  DECLARE _findNext
+  WITH x: Z, v: val, b: val, p: val, n: val, tp: val, 
+       pa: val, pb: val, px: Z, pv: val, sh: share, gv: globals
+  PRE [ tptr tvoid, tptr (tptr tvoid), tint ]
+          PROP (writable_share sh; is_pointer_or_null pa; is_pointer_or_null pb)
+          PARAMS (b; Vint (Int.repr x); v) GLOBALS (gv)
+          SEP (data_at sh (t_struct_tree_t) (p, n) b;
+               field_at sh (t_struct_tree_t) [StructField _t] tp p;
+               data_at sh t_struct_tree (Vint (Int.repr px), (pv, (pa, pb))) tp)
+  POST [ tint ]
+  EX (succ: bool), EX (n' : val),
+         PROP (match succ with
+               | true => ((n' = pa /\ (Z.lt (Int.signed (Int.repr x)) (Int.signed (Int.repr px)))) \/
+                         (n' = pb /\ (Z.lt (Int.signed (Int.repr px)) (Int.signed (Int.repr x)))))
+               | false => (n' = p /\ Int.signed (Int.repr x) = Int.signed (Int.repr px))
+               end)
+        LOCAL (temp ret_temp (Vint (if succ then Int.one else Int.zero)))
+        SEP (match succ with
+             | true =>
+               (data_at sh (t_struct_tree) (p, n') b *
+               field_at sh (t_struct_tree_t) [StructField _t] tp p *
+               data_at sh t_struct_tree (Vint (Int.repr px), (pv, (pa, pb))) tp)
+             | false =>
+               (data_at sh (t_struct_tree) (p, n) b *
+               field_at sh (t_struct_tree_t) [StructField _t] tp p *
+               data_at sh t_struct_tree (Vint (Int.repr px), (pv, (pa, pb))) tp)
+             end).
+
+(*
 #[export] Instance pointer_lock : Ghost := discrete_PCM (val * val * range).
 Definition ghost_info : Type := (key * val)%type.
 
@@ -41,7 +151,8 @@ Class NodeRep : Type := {
   node_rep_R : val -> range -> option (option ghost_info) -> gname -> mpred
   }.
 
-#[global]Instance my_specific_tree_rep : NodeRep := {
+
+#[export]Instance my_specific_tree_rep : NodeRep := {
   node_rep_R := fun tp r g_info g =>
     EX (ga gb : gname), EX (x : Z), EX (v pa pb : val), EX (locka lockb : val),
       !!(g_info = Some (Some (x, v)) /\ and (Z.le Int.min_signed x) (Z.le x Int.max_signed) /\
@@ -52,4 +163,4 @@ Class NodeRep : Type := {
        malloc_token Ews t_struct_tree tp *
        in_tree g ga pa locka * in_tree g gb pb lockb
 }.
-
+*)
