concurrency/Modular/dataStruct.v
@@ -1,0 +1,61 @@
+Require Import VST.concurrency.conclib.
+Require Import VST.floyd.proofauto.
+Require Import VST.atomics.general_locks.
+Require Import Coq.Sets.Ensembles.
+Require Import bst.puretree.
+(* Require Import bst.give_up_template. 
+ Require Import bst.bst_inst. *)
+Require Import VST.atomics.verif_lock_atomic.
+Require Import VST.floyd.library.
+
+(*
+#[export] Instance CompSpecs : compspecs. make_compspecs prog. Defined.
+Definition Vprog : varspecs.  mk_varspecs prog. Defined.
+*)
+
+(* Definition t_struct_tree := Tstruct _node noattr.
+Definition t_struct_tree_t := Tstruct _node_t noattr. 
+Definition t_struct_node := Tstruct _node_t noattr.
+Definition t_struct_pn := Tstruct _pn noattr. *)
+
+Definition number2Z (x : number) : Z :=
+  match x with
+    | Finite_Integer y => y
+    | Neg_Infinity => Int.min_signed
+    | Pos_Infinity => Int.max_signed
+  end.
+
+(* FOUND = 0, NOTFOUND = 1, NULLNEXT = 2 (NULLNEXT = NULL || NEXT ) *)
+(* FOUND = F, NOTFOUND = NF, NULLNEXT = NN *)
+Inductive enum : Type := F | NF | NN.
+
+Definition enums x : val :=
+  match x with
+  | F => Vint Int.zero
+  | NF => Vint Int.one
+  | NN => Vint (Int.repr 2%Z)
+  end.
+
+#[global] Instance enum_inhabited : Inhabitant (enum).
+Proof.
+  unfold Inhabitant; apply F.
+Defined.
+
+#[export] Instance pointer_lock : Ghost := discrete_PCM (val * val * range).
+Definition ghost_info : Type := (key * val)%type.
+
+(* This allows the range to be outdated while the ghost_info may be present or absent. *)
+#[export] Instance node_ghost : Ghost := prod_PCM pointer_lock (exclusive_PCM (option ghost_info)).
+Notation node_info := (@G node_ghost).
+
+Definition in_tree (g: gname) (g1 : gname) (pn: val) (lock: val):=
+      ghost_snap (P := gmap_ghost (K := gname)(A := discrete_PCM (val * val)) )
+        ({[g1 := (pn, lock)]}) g.
+
+Lemma in_tree_duplicate g gin pn lock:
+  in_tree g gin pn lock |-- in_tree g gin pn lock * in_tree g gin pn lock.
+Proof. by rewrite - bi.persistent_sep_dup. Qed.
+
+Section NodeRep.
+  Class NodeRep : Type := { node_rep_R : val -> range -> option (option ghost_info) -> gname -> mpred}.
+End NodeRep.
